mod .gitignore, Spilling: proof of stupSpill

theories/Spilling.v
@@ -1,18 +1,11 @@
 Require Import List Map Env AllInRel Exp MoreExp.
-Require Import IL Annotation InRel AutoIndTac Liveness.
-Require Import Bisim BisimTactics.
-
-
-Inductive stmt : Type :=
- | stmtLet : var -> exp -> stmt -> stmt
- | stmtReturn : exp -> stmt
- | stmtIf : exp -> stmt -> stmt -> stmt.
+Require Import IL Annotation InRel AutoIndTac Liveness LabelsDefined.
+Require Import SimI.
 
 
 (* TODO: Read IL/Annotation.v which defines annotations for programs
          and figure out which type X to choose such that ann X is
          the type of spilling annotations. *)
-(* ann (set var * set var)*)
 
 (* TODO: define the algorithm that takes a program and a spilling
          annotation and produces the spilled program
@@ -42,61 +35,139 @@ end.
 (* TODO: read Liveness.v and figure out the type of the correctness
          predicate for spilling *)
 Inductive spill_sound : nat -> (list (set var * set var)) -> (set var * set var) -> stmt -> ann (set var * set var) -> Prop :=
+
 | SpillLet k Λ R M Sp L K Kx sl x e s
-: spill_sound k Λ ({x;(R\K ∪ L)\Kx }, M ∪ Sp) s sl
-->Exp.freeVars e ⊆ R\K ∪ L
-->cardinal (R\K ∪ L) <= k
-->cardinal ({x;((R\K) ∪ L)\Kx }) <= k
-->spill_sound k Λ (R,M) (stmtLet x e s) (ann1 (Sp,L) sl)
+: spill_sound k Λ ({x;(R\K ∪ L)\Kx }, Sp ∪ M) s sl
+  -> Exp.freeVars e ⊆ R\K ∪ L
+  -> cardinal (R\K ∪ L) <= k
+  -> cardinal ({x;((R\K) ∪ L)\Kx }) <= k
+  -> spill_sound k Λ (R,M) (stmtLet x e s) (ann1 (Sp,L) sl)
+
 | SpillReturn k Λ R M Sp L K e
 : Exp.freeVars e ⊆ R\K ∪ L
- -> cardinal ((R\K) ∪ L) <= k
- ->spill_sound k Λ (R,M) (stmtReturn e) (ann0 (Sp,L))
+  -> cardinal ((R\K) ∪ L) <= k
+  -> spill_sound k Λ (R,M) (stmtReturn e) (ann0 (Sp,L))
+
 | SpillIf k Λ R M Sp L K sl_s sl_t e s t
 : Exp.freeVars e ⊆ R\K ∪ L
- -> cardinal (R\K ∪ L) <= k
- -> spill_sound k Λ (R\K ∪ L, M ∪ Sp) s sl_s
- -> spill_sound k Λ (R\K ∪ L, M ∪ Sp) t sl_t
- -> spill_sound k Λ (R,M) (stmtIf e s t) (ann2 (Sp,L) sl_s sl_t)
+  -> cardinal (R\K ∪ L) <= k
+  -> spill_sound k Λ (R\K ∪ L, Sp ∪ M) s sl_s
+  -> spill_sound k Λ (R\K ∪ L, Sp ∪ M) t sl_t
+  -> spill_sound k Λ (R,M) (stmtIf e s t) (ann2 (Sp,L) sl_s sl_t)
+
+| SpillApp k Λ R M Sp L K f Y R_f M_f
+: cardinal (R\K ∪ L) <= k
+  -> get Λ (counted f) (R_f,M_f)
+  -> R_f ⊆ R\K ∪ L
+  -> M_f ⊆ Sp ∪ M
+    -> spill_sound k Λ (R,M) (stmtApp f Y) (ann0 (Sp,L))
+
+| SpillFun k Λ R M Sp L K s t sl_s sl_t Z
+: cardinal (R\K ∪ L) <= k
+  -> spill_sound k (getAnn sl_s::Λ) (getAnn sl_s) s sl_s 
+  -> spill_sound k (getAnn sl_s::Λ) (R\K ∪ L, M ∪ Sp) t sl_t
+    -> spill_sound k Λ (R,M) (stmtFun ((Z,s)::nil) t)
+                   (annF (Sp,L) (sl_s::nil) sl_t)
+.
+
+Inductive fv_e_bounded : nat -> stmt -> Prop :=
+
+| BoundLet k x e s
+: cardinal (Exp.freeVars e) <= k
+  -> fv_e_bounded k s
+  -> fv_e_bounded k (stmtLet x e s)
+
+| BoundReturn k e
+: cardinal (Exp.freeVars e) <= k
+  -> fv_e_bounded k (stmtReturn e)
+
+| BoundIf k e s t
+: cardinal (Exp.freeVars e) <= k
+  -> fv_e_bounded k s
+  -> fv_e_bounded k t
+  -> fv_e_bounded k (stmtIf e s t)
+
+| BoundApp k f Y
+: fv_e_bounded k (stmtApp f Y)
+
+| BoundFun k Z s t 
+: fv_e_bounded k (stmtFun ((Z,s)::nil) t)
 .
 
 Fixpoint stupSpill (R : set var) (s : stmt) : ann (set var * set var) := 
-(*fix stSp (R : set var) (s : stmt) : ann (set var * set var) := *)
 match s with
-| stmtLet x e t => ann1 (R, Exp.freeVars e) (stupSpill ((Exp.freeVars e) ∪ singleton x) t)
+| stmtLet x e t => ann1 (R, Exp.freeVars e)
+                        (stupSpill (singleton x) t)
 | stmtReturn e => ann0 (R, Exp.freeVars e)
-| stmtIf e t v => ann2 (R, Exp.freeVars e) (stupSpill (Exp.freeVars e) t) (stupSpill (Exp.freeVars e) v)
-(*| stmtApp f xs => ann0 (R, ∅)*)
-(*| stmtFun f xs t v => ann2 (R, ∅) (stSp ∅ t) (stSp ∅ v)*)
-(*| _ => ann0 (∅,∅)*)
-end
-(*) ∅ s*)
-.
-
-Fixpoint freeVars (s:stmt) : set var :=
-  match s with
-    | stmtLet x e s0 => (freeVars s0 \ singleton x) ∪ Exp.freeVars e
-    | stmtIf e s1 s2 => freeVars s1 ∪ freeVars s2 ∪ Exp.freeVars e
-    | stmtReturn e => Exp.freeVars e
-  end.
-
-Set Implicit Arguments.
-Unset Strict Implicit.
-
-Lemma stupSpill_sat_spillSound (k:nat) (s:stmt) :
-(* forall e : exp in s, cardinal (Exp.freeVars) <= k*)
-freeVars s =  ∅ -> 
-spill_sound k nil (∅,∅) s (stupSpill ∅ s).
-assert (forall R M, freeVars s ⊆ R ∪ M -> spill_sound k nil (R,M) s (stupSpill R s)).
- - intros R M subs.
-   induction s.
-   + simpl. simpl in subs. admit.
-   + admit.
-   + admit.
- - intros. apply (H ∅ ∅). rewrite H0. admit.
+| stmtIf e t v => ann2 (R, Exp.freeVars e)
+                       (stupSpill ∅ t) 
+                       (stupSpill ∅ v)
+| stmtApp f Y => ann0 (R, ∅)
+| stmtFun ((Z,t)::nil) v => annF (R, ∅) (stupSpill ∅ t::nil) (stupSpill ∅ v)
+| _ => ann0 (∅,∅)
+end.
 
 
- destruct. assert (exists K, K ⊆ R /\ cardinal K = cardinal (Exp.freeVars e)).
+
+
+Lemma stupSpill_sat_spillSound (k:nat) (s:stmt) (R R' M : set var) Λ Lv ZL alv :
+k > 0
+-> freeVars s ⊆ R' ∪ M
+-> R' ⊆ R
+-> fv_e_bounded k s
+-> live_sound Imperative ZL Lv s alv
+-> getAnn alv ⊆ R' ∪ M 
+-> PIR2 (fun RMf G => fst RMf [=] ∅ /\ snd RMf [=] G) Λ (Lv \\ ZL)
+-> spill_sound k Λ (R,M) s (stupSpill R' s).
+
+Proof.
+  intros knotzero subs.
+  general induction s; invt fv_e_bounded; invt live_sound; simpl in *.
+   - simpl. eapply SpillLet with (K := R)(Kx := Exp.freeVars e).
+     + eapply IHs; eauto.
+       * rewrite <- subs. clear_all. cset_tac. decide (x === a); eauto. 
+       * clear_all. eauto with cset.
+       * rewrite <- H2. clear - H14. cset_tac. decide (x === a); eauto with cset.
+           right. assert (forall y, y ∈ (getAnn al \ singleton x) -> y ∈ lv); 
+                eauto with cset.
+           eapply H0. cset_tac.
+     + eauto with cset.
+     + assert (R \ R ∪ Exp.freeVars e [=] Exp.freeVars e). 
+       * cset_tac.
+       * rewrite H4. auto.
+     + assert ({x; R \ R ∪ Exp.freeVars e \ Exp.freeVars e} [=] singleton x).
+       * clear_all. cset_tac. 
+       * rewrite H4. rewrite singleton_cardinal. auto.
+   - eapply SpillIf with (K := R). 
+     + eauto with cset.
+     + assert (R \ R ∪ Exp.freeVars e [=] Exp.freeVars e). cset_tac.
+       rewrite H4. auto.
+     + eapply IHs1; eauto with cset.
+       rewrite <- subs. clear_all. cset_tac.
+     + eapply IHs2; eauto with cset.
+       rewrite <- subs. clear_all. cset_tac.
+   - assert (get (Lv \\ ZL) (labN l) (blv \ of_list Z)).
+     + eapply zip_get_eq; eauto.
+     + PIR2_inv. destruct x as [R_f M_f]; simpl in *.
+       eapply SpillApp with (K := R); eauto.
+       * assert (R\R ∪ ∅ [=] ∅) as empty. 
+           clear_all. cset_tac. 
+           rewrite empty. rewrite empty_cardinal. omega.
+       * rewrite H10. eauto with cset.
+       * rewrite H12. rewrite H8. eauto.
+   - eapply SpillReturn with (K := R).
+     + eauto with cset.
+     + assert (R \ R ∪ Exp.freeVars e [=] Exp.freeVars e).
+       * cset_tac.
+       * rewrite H4. auto.
+   - eapply SpillFun with (K := R); simpl in *.
+     + assert (R\R ∪ ∅ [=] ∅) as empty. 
+       * clear_all. cset_tac. 
+       * rewrite empty. rewrite empty_cardinal. omega.
+     + admit.
+     + admit.    
+
+Qed.
 
 
 
